src/spec/TLS13.ConnectionState.Lemmas.fst
@@ -3002,6 +3002,32 @@ let lemma_server_application_ready_stable_x25519_key_share_projection
 
 #pop-options
 
+#push-options "--fuel 2 --ifuel 2 --z3rlimit 20"
+let lemma_client_handshake_stable_x25519_key_share_projection
+  (st:connection_state)
+  : Lemma
+      (requires
+        connection_state_consistent st /\
+        st.cs_model.model_config.config_role == ClientEndpoint /\
+        Some? st.cs_model.model_handshake.hs_keys.ks_shared_secret)
+      (ensures stable_client_x25519_key_share_projection st)
+=
+  lemma_connection_state_consistent_client_x25519_reachable_shape st
+
+let lemma_server_handshake_stable_x25519_key_share_projection
+  (st:connection_state)
+  : Lemma
+      (requires
+        connection_state_consistent st /\
+        st.cs_model.model_config.config_role == ServerEndpoint /\
+        Some? st.cs_model.model_handshake.hs_keys.ks_shared_secret /\
+        ControlHandshaking? st.cs_model.model_control /\
+        st.cs_model.model_control =!= ControlHandshaking HsClientHelloReceived)
+      (ensures stable_server_x25519_key_share_projection st)
+=
+  lemma_connection_state_consistent_server_x25519_reachable_shape st
+#pop-options
+
 let lemma_record_read_key_schedule_projection_client_projection
   (model:connection_model)
   : Lemma
